@prefix : <https://w3id.org/won/model#> .
@prefix dc: <http://purl.org/dc/elements/1.1/> .
@prefix gr: <http://purl.org/goodrelations/v1#> .
@prefix owl: <http://www.w3.org/2002/07/owl#> .
@prefix rdf: <http://www.w3.org/1999/02/22-rdf-syntax-ns#> .
@prefix xml: <http://www.w3.org/XML/1998/namespace> .
@prefix xsd: <http://www.w3.org/2001/XMLSchema#> .
@prefix oslc: <http://open-services.net/ns/core#> .
@prefix rdfs: <http://www.w3.org/2000/01/rdf-schema#> .
@prefix sioc: <http://rdfs.org/sioc/types#> .
@prefix schema_org: <http://schema.rdfs.org/all#> .
@base <https://w3id.org/won/model> .

<https://w3id.org/won/model> rdf:type owl:Ontology ;
                                    owl:versionIRI <https://w3id.org/won/model/1.0> ;
                                    dc:title "Web of Needs Ontology" ;
                                    rdfs:comment "Ontology for the Web of Needs data model."@en ;
                                    dc:date "2013-12-13"^^xsd:date ;
                                    dc:creator "Florian Kleedorfer" ,
                                               "Fabian Salcher" .

#################################################################
#    Object Properties
#################################################################

###  https://w3id.org/won/model#hasAdditionalData
:hasAdditionalData rdf:type owl:ObjectProperty ;
                   rdfs:range owl:Thing ;
                   rdfs:comment "Contains additional information in form of an RDF graph about an event."^^xsd:string ;
                   rdfs:isDefinedBy <https://w3id.org/won/model> .


###  https://w3id.org/won/model#hasBrokerUri
:hasBrokerUri rdf:type owl:ObjectProperty ;
              rdfs:domain :WonOverActiveMq ;
              rdfs:comment "Specifies the ActiveMQ broker URI to be used to contact the need."@en ;
              rdfs:isDefinedBy <https://w3id.org/won/model> .


###  https://w3id.org/won/model#hasConnectionState
:hasConnectionState rdf:type owl:ObjectProperty ,
                             owl:FunctionalProperty ;
                    rdfs:domain :Connection ;
                    rdfs:range :ConnectionState ;
                    rdfs:comment "Indicates the state in which the Connection object is."@en ;
                    rdfs:isDefinedBy <https://w3id.org/won/model> .


###  https://w3id.org/won/model#hasConnections
:hasConnections rdf:type owl:ObjectProperty ;
                rdfs:domain :Need ;
                rdfs:range :ConnectionContainer ;
                rdfs:comment "Links the Need object to its connections."@en ;
                rdfs:isDefinedBy <https://w3id.org/won/model> .


###  https://w3id.org/won/model#hasEventContainer
:hasEventContainer rdf:type owl:ObjectProperty ,
                            owl:FunctionalProperty ;
                   rdfs:domain :Connection ;
                   rdfs:range :EventContainer ;
                   rdfs:comment "Links the Connection object to a container containing connection events (messages)."@en ;
                   rdfs:isDefinedBy <https://w3id.org/won/model> .


###  https://w3id.org/won/model#hasFacet
:hasFacet rdf:type owl:ObjectProperty ;
          rdfs:domain :Need ;
          rdfs:range :Facet ;
          rdfs:comment "Indicates that a need or connection supports the specified facet (=behavior)."@en ;
          rdfs:isDefinedBy <https://w3id.org/won/model> .

		  
###  https://w3id.org/won/model#hasDefaultFacet
:hasDefaultFacet rdf:type owl:ObjectProperty ;
          rdfs:domain :Need ;
          rdfs:range :Facet ;
          rdfs:comment "Indicates the facet to connect to by default."@en ;
          rdfs:isDefinedBy <https://w3id.org/won/model> .

		  

###  https://w3id.org/won/model#hasFlag
:hasFlag rdf:type owl:ObjectProperty ;
         rdfs:domain :Need ;
         rdfs:range :Flag ;
         rdfs:comment "Links a Need to its Flags"@en ;
         rdfs:isDefinedBy <https://w3id.org/won/model> .


###  https://w3id.org/won/model#hasMatchingContext
:hasFlag rdf:type owl:ObjectProperty ;
         rdfs:domain :Need ;
         rdfs:range xsd:String ;
         rdfs:comment "Specifies a 'matching context' for the Need. Matchers should only send hints to this Need if the counterpart specifies the same matching context. If no matching context is specified, matching is not restricted, and matchers may send hints with counterparts that do specify matching contexts."@en ;
         rdfs:isDefinedBy <https://w3id.org/won/model> .


###  https://w3id.org/won/model#hasLocation
:hasLocation rdf:type owl:ObjectProperty ;
             rdfs:range :LocationSpecification ;
             rdfs:comment "Links a NeedDescription entity to a description of its location."@en ;
             rdfs:isDefinedBy <https://w3id.org/won/model> .


###  https://w3id.org/won/model#hasMatcherProtocolEndpoint
:hasMatcherProtocolEndpoint rdf:type owl:ObjectProperty ;
                            rdfs:comment "Points to the matcherProtocol webservice endpoint of the need. I.e., matchers can communicate with the need through this endpoint."@en ;
                            rdfs:isDefinedBy <https://w3id.org/won/model> .


###  https://w3id.org/won/model#hasNeedProtocolEndpoint
:hasNeedProtocolEndpoint rdf:type owl:ObjectProperty ;
                         rdfs:subPropertyOf owl:topObjectProperty ;
                         rdfs:comment "Points to the needProtocol webservice endpoint of the need. I.e., won nodes can communicate with the need through this endpoint."@en ;
                         rdfs:isDefinedBy <https://w3id.org/won/model> .


###  https://w3id.org/won/model#hasOriginator
:hasOriginator rdf:type owl:ObjectProperty ,
                        owl:InverseFunctionalProperty ;
               rdfs:comment "The entity (Need, Connection, or Service - eg. matching service) that originated the event."@en ;
               rdfs:isDefinedBy <https://w3id.org/won/model> .


###  https://w3id.org/won/model#hasOwner
:hasOwner rdf:type owl:ObjectProperty ,
                   owl:FunctionalProperty ;
          rdfs:domain :Need ;
          rdfs:comment "Specifies who controls the need."@en ;
          rdfs:isDefinedBy <https://w3id.org/won/model> .


###  https://w3id.org/won/model#hasOwnerProtocolEndpoint
:hasOwnerProtocolEndpoint rdf:type owl:ObjectProperty ;
                          rdfs:comment "Points to the ownerProtocol webservice endpoint of the need. I.e., owner applications can communicate with the need through this endpoint."@en ;
                          rdfs:isDefinedBy <https://w3id.org/won/model> .


###  https://w3id.org/won/model#hasRemoteConnection
:hasRemoteConnection rdf:type owl:ObjectProperty ,
                              owl:FunctionalProperty ,
                              owl:InverseFunctionalProperty ,
                              owl:SymmetricProperty ;
                     rdfs:domain :Connection ;
                     rdfs:range :Connection ;
                     rdfs:comment "Links a Connection object to its remote counterpart."@en ;
                     rdfs:isDefinedBy <https://w3id.org/won/model> .


###  https://w3id.org/won/model#hasRemoteFacet
:hasRemoteFacet rdf:type owl:ObjectProperty ;
                rdfs:comment "Indicates that a remote need or remote connection supports the specified facet (=behavior) or specifies the remote facet to connect with."@en ;
                rdfs:isDefinedBy <https://w3id.org/won/model> .


###  https://w3id.org/won/model#hasRemoteNeed
:hasRemoteNeed rdf:type owl:ObjectProperty ;
               rdfs:domain :Connection ;
               rdfs:range :Need ;
               rdfs:comment "links a Connection to its remote Need. The remote Need is the one holding the  remoteConnection."@en ;
               rdfs:isDefinedBy "https://w3id.org/won/model"@en .


###  https://w3id.org/won/model#hasTag
:hasTag rdf:type owl:ObjectProperty ;
        rdfs:range xsd:string .


###  https://w3id.org/won/model#hasTimeSpecification
:hasTimeSpecification rdf:type owl:ObjectProperty ;
                      rdfs:range :TimeSpecification ;
                      rdfs:comment "Specifies when the Need object is available."@en ;
                      rdfs:isDefinedBy <https://w3id.org/won/model> .


###  https://w3id.org/won/model#isInState
:isInState rdf:type owl:ObjectProperty ,
                    owl:FunctionalProperty ;
           rdfs:domain :Need ;
           rdfs:range :NeedState ;
           rdfs:comment "Defines the Need object's state."@en ;
           rdfs:isDefinedBy <https://w3id.org/won/model> .


###  https://w3id.org/won/model#seeks
:seeks rdf:type owl:ObjectProperty ;
       rdfs:domain :Need ;
       rdfs:comment """This optional property is one of the two properties that defines the content of every need (the other is the \"is\" property). It is used to describe that part of the content that is
sought to fulfill the need in contrast to the part that is available.""" ;
       rdfs:isDefinedBy <https://w3id.org/won/model> .


###  https://w3id.org/won/model#supportsWonProtocolImpl
:supportsWonProtocolImpl rdf:type owl:ObjectProperty ;
                         rdfs:domain :Need ;
                         rdfs:range :WonProtocol ;
                         rdfs:comment "Connects a Need object with a description of a WON protocol it supports."@en ;
                         rdfs:isDefinedBy <https://w3id.org/won/model> .

#################################################################
#    Data properties
#################################################################

###  http://purl.org/dc/terms#created
<http://purl.org/dc/terms#created> rdf:type owl:DatatypeProperty ;
                                   rdfs:subPropertyOf owl:topDataProperty ;
                                   rdfs:isDefinedBy <https://w3id.org/won/model> .


###  http://purl.org/dc/terms/title
<http://purl.org/dc/terms/title> rdf:type owl:DatatypeProperty .


###  https://w3id.org/won/model#hasActiveMQNeedProtocolQueueName
:hasActiveMQNeedProtocolQueueName rdf:type owl:DatatypeProperty ;
                                  rdfs:comment "Name of the ActiveMQ queue used for the need protocol."@en ;
                                  rdfs:isDefinedBy <https://w3id.org/won/model> .


###  https://w3id.org/won/model#hasActiveMQOwnerProtocolQueueName
:hasActiveMQOwnerProtocolQueueName rdf:type owl:DatatypeProperty ;
                                   rdfs:comment "Name of the ActiveMQ queue used for the owner protocol."@en ;
                                   rdfs:isDefinedBy <https://w3id.org/won/model> .


###  https://w3id.org/won/model#hasEndTime
:hasEndTime rdf:type owl:DatatypeProperty ,
                     owl:FunctionalProperty ;
            rdfs:domain :TimeSpecification ;
            rdfs:range xsd:dateTime ;
            rdfs:comment "The end time as an xsd:dateTime."@en ;
            rdfs:isDefinedBy <https://w3id.org/won/model> .


###  https://w3id.org/won/model#hasRecursIn
:hasRecursIn rdf:type owl:DatatypeProperty ,
                      owl:FunctionalProperty ;
             rdfs:domain :TimeSpecification ;
             rdfs:range xsd:duration ;
             rdfs:comment "If set, specifies the interval of recurrence measured from the startTime, in xsd:duration."@en ;
             rdfs:isDefinedBy <https://w3id.org/won/model> .


###  https://w3id.org/won/model#hasRecursInfiniteTimes
:hasRecursInfiniteTimes rdf:type owl:DatatypeProperty ,
                                 owl:FunctionalProperty ;
                        rdfs:domain :TimeSpecification ;
                        rdfs:range xsd:boolean ;
                        rdfs:comment "Indicates that the TimeSpecification is repeated until the end of time."@en ;
                        rdfs:isDefinedBy <https://w3id.org/won/model> .


###  https://w3id.org/won/model#hasRecursTimes
:hasRecursTimes rdf:type owl:DatatypeProperty ,
                         owl:FunctionalProperty ;
                rdfs:domain :TimeSpecification ;
                rdfs:range xsd:integer ;
                rdfs:comment "Specifies how often the interval recurs."@en ;
                rdfs:isDefinedBy <https://w3id.org/won/model> .


###  https://w3id.org/won/model#hasStartTime
:hasStartTime rdf:type owl:DatatypeProperty ,
                       owl:FunctionalProperty ;
              rdfs:domain :TimeSpecification ;
              rdfs:range xsd:dateTime ;
              rdfs:comment "The start time as an xsd:dateTime."@en ;
              rdfs:isDefinedBy <https://w3id.org/won/model> .

###  https://w3id.org/won/model#doNotMatchBefore
:doNotMatchBefore rdf:type owl:DatatypeProperty ,
                     owl:FunctionalProperty ;
            rdfs:domain :Need ;
            rdfs:range xsd:dateTime ;
            rdfs:comment "Indicates that matchers should not use this need for matching before the specified xsd:dateTime."@en ;
            rdfs:isDefinedBy <https://w3id.org/won/model> .

###  https://w3id.org/won/model#doNotMatchAfter
:doNotMatchAfter rdf:type owl:DatatypeProperty ,
                     owl:FunctionalProperty ;
            rdfs:domain :Need ;
            rdfs:range xsd:dateTime ;
            rdfs:comment "Indicates that matchers should not use this need for matching after the specified xsd:dateTime."@en ;
            rdfs:isDefinedBy <https://w3id.org/won/model> .

###  https://w3id.org/won/model#hasTag
:hasTag rdf:type owl:DatatypeProperty .


###  https://w3id.org/won/model#hasTimeStamp
:hasTimeStamp rdf:type owl:DatatypeProperty ,
                       owl:FunctionalProperty ;
              rdfs:range xsd:dateTime ;
              rdfs:comment "The time and date when the event occurred."@en ;
              rdfs:isDefinedBy <https://w3id.org/won/model> .


###  http://www.w3.org/2003/01/geo/wgs84_pos#latitude
<http://www.w3.org/2003/01/geo/wgs84_pos#latitude> rdf:type owl:DatatypeProperty ,
                                                            owl:FunctionalProperty ;
                                                   rdfs:domain <http://www.w3.org/2003/01/geo/wgs84_pos#Point> ;
                                                   rdfs:range xsd:float ;
                                                   rdfs:isDefinedBy <https://w3id.org/won/model> .


###  http://www.w3.org/2003/01/geo/wgs84_pos#longitude
<http://www.w3.org/2003/01/geo/wgs84_pos#longitude> rdf:type owl:DatatypeProperty ,
                                                             owl:FunctionalProperty ;
                                                    rdfs:domain <http://www.w3.org/2003/01/geo/wgs84_pos#Point> ;
                                                    rdfs:range xsd:float .


#################################################################
#    Classes
#################################################################

###  https://w3id.org/won/model#Connection
:Connection rdf:type owl:Class ;
            rdfs:comment "Represents a Connection to between two Needs. Whenever two Needs are connected, each Need creates a dedicated Connection object which encapsulate all information about the connection."@en ;
            rdfs:isDefinedBy <https://w3id.org/won/model> .


###  https://w3id.org/won/model#ConnectionContainer
:ConnectionContainer rdf:type owl:Class ;
                     rdfs:subClassOf <http://www.w3.org/ns/ldp#CompositeContainer> ;
                     rdfs:comment "Container for Connections."@en ;
                     rdfs:isDefinedBy <https://w3id.org/won/model> .


###  https://w3id.org/won/model#ConnectionState
:ConnectionState rdf:type owl:Class ;
                 rdfs:comment "A Connection's state."@en ;
                 rdfs:isDefinedBy <https://w3id.org/won/model> .


###  https://w3id.org/won/model#EventContainer
:EventContainer rdf:type owl:Class ;
                rdfs:subClassOf <http://www.w3.org/ns/ldp#CompositeContainer> ;
                rdfs:comment "Container for Events."@en ;
                rdfs:isDefinedBy <https://w3id.org/won/model> .


###  https://w3id.org/won/model#Facet
:Facet rdf:type owl:Class ;
       rdfs:comment "Facets are behaviors a Need can choose to support. Connections have a Facet; Needs can be connected through multiple Connections if they have different Facets."@en ;
       rdfs:isDefinedBy <https://w3id.org/won/model> .


###  https://w3id.org/won/model#Flag
:Flag rdf:type owl:Class ;
      rdfs:comment "Superclass of all Flags a need can have."@en ;
      rdfs:isDefinedBy <https://w3id.org/won/model> .


###  https://w3id.org/won/model#LocationSpecification
:LocationSpecification rdf:type owl:Class ;
                       rdfs:comment "Specifies where a Need is available."@en ;
                       rdfs:isDefinedBy <https://w3id.org/won/model> .

###  https://w3id.org/won/model#Need
:Need rdf:type owl:Class ;
      rdfs:comment """A need is an online entity controlled by a person or organization. Its purpose is to be connected to other such needs via Connections, so it can be said that it represents the need to interact with others.
It specifies a content - what the need is about, which may be something that is offered for sale, sought for rental etc."""@en ;
      rdfs:isDefinedBy <https://w3id.org/won/model> ;
      rdfs:label "Need" .


###  https://w3id.org/won/model#NeedState
:NeedState rdf:type owl:Class ;
           rdfs:comment "The Need's state."@en ;
           rdfs:isDefinedBy <https://w3id.org/won/model> .


###  https://w3id.org/won/model#Region
:Region rdf:type owl:Class ;
        rdfs:subClassOf :LocationSpecification ;
        rdfs:isDefinedBy <https://w3id.org/won/model> .


###  https://w3id.org/won/model#TimeSpecification
:TimeSpecification rdf:type owl:Class ;
                   rdfs:comment "Specifies when a Need is available. Matching services should try to find Needs with TimeSpecifications that overlap with this needs' TimeSpecifications."@en ;
                   rdfs:isDefinedBy <https://w3id.org/won/model> .


###  https://w3id.org/won/model#WonOverActiveMq
:WonOverActiveMq rdf:type owl:Class ;
                 rdfs:subClassOf :WonProtocol ;
                 rdfs:comment "The Web of Needs protocol implementation that uses ActiveMQ."@en ;
                 rdfs:isDefinedBy <https://w3id.org/won/model> .


###  https://w3id.org/won/model#WonOverSoapWs
:WonOverSoapWs rdf:type owl:Class ;
               rdfs:subClassOf :WonProtocol ;
               rdfs:comment "The Web of Needs Protocol implelementation that uses SOAP Webservices."@en ;
               rdfs:isDefinedBy <https://w3id.org/won/model> .


###  https://w3id.org/won/model#WonProtocol
:WonProtocol rdf:type owl:Class ;
             rdfs:comment """Superclass for Web of Needs protocol implementations."""@en ;
             rdfs:isDefinedBy <https://w3id.org/won/model> .


###  http://www.w3.org/2003/01/geo/wgs84_pos#Point
<http://www.w3.org/2003/01/geo/wgs84_pos#Point> rdf:type owl:Class ;
                                                rdfs:subClassOf :LocationSpecification .


###  http://www.w3.org/ns/ldp#CompositeContainer
<http://www.w3.org/ns/ldp#CompositeContainer> rdf:type owl:Class ;
                                              rdfs:isDefinedBy <https://w3id.org/won/model> .


#################################################################
#    Individuals
#################################################################

###  https://w3id.org/won/model#Active
:Active rdf:type owl:NamedIndividual ,
                 :NeedState ;
        rdfs:comment "The active state. "@en ;
        rdfs:isDefinedBy <https://w3id.org/won/model> .


###  https://w3id.org/won/model#Closed
:Closed rdf:type owl:NamedIndividual ,
                 :ConnectionState ;
        rdfs:comment "The closed state. No Messages are forwarded in this state. Re-opening a connection is possbile."@en ;
        rdfs:isDefinedBy <https://w3id.org/won/model> .


###  https://w3id.org/won/model#Connected
:Connected rdf:type owl:NamedIndividual ,
                    :ConnectionState ;
           rdfs:comment "The connected state. Messages are forwarded to/from the owner."@en ;
           rdfs:isDefinedBy <https://w3id.org/won/model> .


###  https://w3id.org/won/model#NoHintForMe
:NoHintForMe rdf:type owl:NamedIndividual, :Flag;
            rdfs:comment "A Need specifying this flag indicates that matchers should not send Hint messages to that Need. If the NoHintForCounterpart flag is also present, matchers should disregard this need completely."@en ;
            rdfs:isDefinedBy <https://w3id.org/won/model> .

###  https://w3id.org/won/model#NoHintForCounterpart
:NoHintForCounterpart rdf:type owl:NamedIndividual, :Flag;
            rdfs:comment "A Need specifying this flag indicates that matchers should not send Hint messages to the counterpart in case of a match. If the NoHintForMe flag is also present, matchers should disregard this need completely."@en ;
            rdfs:isDefinedBy <https://w3id.org/won/model> .

###  https://w3id.org/won/model#WhatsAround
:WhatsAround rdf:type owl:NamedIndividual, :Flag;
            rdfs:comment "A Need specifying this flag indicates that matchers should not match with anything but the location within this need. The intention of this Flag is to simply find other needs around a certain location."@en ;
            rdfs:isDefinedBy <https://w3id.org/won/model> .

###  https://w3id.org/won/model#WhatsNew
:WhatsNew rdf:type owl:NamedIndividual, :Flag;
            rdfs:comment "A Need specifying this flag indicates that matchers should match with anything that is created recently. The intention of this Flag is to simply find other needs created recently."@en ;
            rdfs:isDefinedBy <https://w3id.org/won/model> .

###  https://w3id.org/won/model#GroupFacet
:GroupFacet rdf:type owl:NamedIndividual ,
                     :Facet ;
            rdfs:comment "The group facet. Messages are forwarded to all connections with this facet."@en ;
            rdfs:isDefinedBy <https://w3id.org/won/model> .


###  https://w3id.org/won/model#Inactive
:Inactive rdf:type owl:NamedIndividual ,
                   :NeedState ;
          rdfs:comment "The incative state. Needs do not communicate in this state. Intended to stop receiving messages for something not currently of interest."@en ;
          rdfs:isDefinedBy <https://w3id.org/won/model> .

###  https://w3id.org/won/model#ChatFacet
:ChatFacet rdf:type owl:NamedIndividual ,
                     :Facet ;
            rdfs:comment "The Default facet. All messages and events are forwarded to the owner, no action is taken automatically."@en ;
            rdfs:isDefinedBy <https://w3id.org/won/model> .


###  https://w3id.org/won/model#RequestReceived
:RequestReceived rdf:type owl:NamedIndividual ,
                          :ConnectionState ;
                 rdfs:comment "Half-open state. The connection has been opened by the remote counterpart but not yet been accepted by the local end."@en ;
                 rdfs:isDefinedBy <https://w3id.org/won/model> .


###  https://w3id.org/won/model#RequestSent
:RequestSent rdf:type owl:NamedIndividual ,
                      :ConnectionState ;
             rdfs:comment "Half-open state. The Connection has been requested by the local end but not yet been accepted by the remote counterpart."@en ;
             rdfs:isDefinedBy <https://w3id.org/won/model> .

###  https://w3id.org/won/model#Suggested
:Suggested rdf:type owl:NamedIndividual ,
                    :ConnectionState ;
           rdfs:comment "Suggested state. The Connection has been created through a Hint Event but not yet been opened by either of the sides."@en ;
           rdfs:isDefinedBy <https://w3id.org/won/model> .


###  https://w3id.org/won/model#UsedForTesting
:UsedForTesting rdf:type owl:NamedIndividual ,
                         :Flag .





#################################################################
#    Annotations
#################################################################

:UsedForTesting rdfs:comment "Flag indicating the need has been created for testing purposes. It should only be matched with other needs flagged with UsedForTesting. The flag is intended to separate real-world needs from those generated for testing the system, so that users are neither spammed nor misled."@en ;
                rdfs:isDefinedBy <https://w3id.org/won/model> .


###  Generated by the OWL API (version 4.2.6.20160910-2108) https://github.com/owlcs/owlapi
